\section{The list Viterbi algorithm}
\label{sec:lva}

Let $\gamma_t(i,j)$ denote the probability of being in state $s_i$ at time $t$, and state $s_j$ at time $t\!+\!1$, 
as well as observations $O_{1:T}$, given the model parameters $\lambda$, \ie
\begin{equation}
\label{eq:gamma}
\begin{aligned}
\gamma_t(i,j) 
&= \sum_{q_{1:t-1,t+2:T}} \p(O_{1:T}, q_{1:t-1}, q_t = s_i, q_{t+1} = s_j, q_{t+2:T} ;\lambda) \\
&= \left[ \sum_{q_{1:t-1}} \p(O_{1:t}, q_{1:t-1}, q_t = s_i ;\lambda) \right] \p(q_{t+1} = s_j |q_t = s_i) \cdot \p(O_{t+1} |q_{t+1} = s_j) 
   \left[ \sum_{q_{t+2:T}} \p(O_{t+2:T}, q_{t+2:T} |q_{t+1} = s_j; \lambda) \right] \\
&= \alpha_t(i) \cdot a_{ij} \cdot b_j(O_{t+1}) \cdot \beta_{t+1}(j) 
   ~~~ \text{(by Eq.~\ref{eq:notebasic}, \ref{eq:alpha} and \ref{eq:beta})}.
\end{aligned}
\end{equation}

While $\gamma_t(i,j)$ is the \emph{marginal} joint probability of all possible observation-state pairs 
$(O_{1:T}, q_{1:t-1} s_i s_j q_{t+2:T})$ given the model,
we can also compute the \emph{maximum} joint probability over all possible observation-state pairs $(O_{1:T}, q_{1:t-1} s_i s_j q_{t+2:T})$, \ie
\begin{equation}
\label{eq:gammat}
\begin{aligned}
\gammat_t(i,j) 
&= \max_{q_{1:t-1,t+2:T}} \p(O_{1:T}, q_{1:t-1}, q_t = s_i, q_{t+1} = s_j, q_{t+2:T} ;\lambda) \\
&= \left\{ \max_{q_{1:t-1}} \p(O_{1:t}, q_{1:t-1}, q_t = s_i ;\lambda) \right\} \p(q_{t+1} = s_j |q_t = s_i) \cdot \p(O_{t+1} |q_{t+1} = s_j) 
   \left\{ \max_{q_{t+2:T}} \p(O_{t+2:T}, q_{t+2:T} |q_{t+1} = s_j; \lambda) \right\} \\
&= \alphat_t(i) \cdot a_{ij} \cdot b_j(O_{t+1}) \cdot \betat_{t+1}(j) 
   ~~~ \text{(by Eq.~\ref{eq:notebasic}, \ref{eq:alphat} and \ref{eq:betat})}.
\end{aligned}
\end{equation}
Similarly, we can fix the state only at time $t$, \ie $q_t = s_i$, 
and the maximum joint probability is
\begin{equation}
\label{eq:gammat0}
\begin{aligned}
\gammat_t(i) 
&= \max_{q_{1:t-1,t+1:T}} \p(O_{1:T}, q_{1:t-1}, q_t = s_i, q_{t+1:T} ;\lambda) \\
&= \left\{ \max_{q_{1:t-1}} \p(O_{1:t}, q_{1:t-1}, q_t = s_i ;\lambda) \right\}  
   \left\{ \max_{q_{t+1:T}} \p(O_{t+1:T}, q_{t+1:T} |q_t = s_i; \lambda) \right\} \\
&= \alphat_t(i) \cdot \betat_t(i) 
   ~~~ \text{(by Eq.~\ref{eq:notebasic}, \ref{eq:alphat} and \ref{eq:betat})}.
\end{aligned}
\end{equation}

Note that the joint probability of state sequence $q_{1:T}$ and observations $O_{1:T}$ is
\begin{equation}
\label{eq:jointdef}
\p(O_{1:T}, q_{1:T} ;\lambda) = \p(q_1) \cdot \p(O_1 |q_1) \left[ \prod_{t=1}^{T-1} \p(q_{t+1} |q_t) \cdot \p(O_{t+1} |q_{t+1}) \right],
\end{equation}
and that
\begin{equation}
\label{eq:jointp}
\begin{aligned}
\frac{\prod_{t=1}^{T-1} \gammat_t(q_t, q_{t+1})} {\prod_{t=2}^{T-1} \gammat_t(q_t)} 
&= \frac{\prod_{t=1}^{T-1} \alphat_t(q_t) \cdot \p(q_{t+1} |q_t) \cdot \p(O_{t+1} |q_{t+1}) \cdot \betat_{t+1}(q_{t+1})}
        {\prod_{t=2}^{T-1} \alphat_t(q_t) \cdot \betat_t(q_t)} 
   ~~~ \text{(by Eq.~\ref{eq:gammat} and \ref{eq:gammat0})} \\
&= \left[ \prod_{t=1}^{T-1} \p(q_{t+1} |q_t) \cdot \p(O_{t+1} |q_{t+1}) \right]
   \frac{ \left[ \prod_{t=1}^{T-1} \alphat_t(q_t) \right] \left[ \prod_{t=2}^T \betat_t(q_t) \right] }
        {\prod_{t=2}^{T-1} \alphat_t(q_t) \cdot \betat_t(q_t)} \\
&= \left[ \prod_{t=1}^{T-1} \p(q_{t+1} |q_t) \cdot \p(O_{t+1} |q_{t+1}) \right] \alphat_1(q_1) \cdot \betat_T(q_T) \\
&= \left[ \prod_{t=1}^{T-1} \p(q_{t+1} |q_t) \cdot \p(O_{t+1} |q_{t+1}) \right] \p(q_1) \cdot \p(O_1 |q_1) \cdot 1 
   ~~~ \text{(by Eq.~\ref{eq:forward-max} and \ref{eq:backward-max})} \\
%&= \p(q_1) \cdot \p(O_1 |q_1) \left[ \prod_{t=1}^{T-1} \p(q_{t+1} |q_t) \cdot \p(O_{t+1} |q_{t+1}) \right] \\
&= \p(O_{1:T}, q_{1:t} ;\lambda) ~~~ \text{(by Eq.~\ref{eq:jointdef})}.
\end{aligned}
\end{equation}

From Eq.~(\ref{eq:gammat}) and (\ref{eq:gammat0}), we note that 
\begin{equation}
\label{eq:maxconsist}
\max_{q_{t+1}} \gammat_t(q_t, q_{t+1}) = \gammat_t(q_t) 
~~~ \text{and} ~~~
\max_{q_t} \gammat_t(q_t, q_{t+1}) = \gammat_{t+1}(q_{t+1}),
\end{equation}
which is known as the \emph{max-consistency} property~\cite{nilsson2001sequentially}.
%and we have the following lemma,

\begin{lemma}
\label{lm:1}
Let $E$ be a set of state sequences given by $E = \{\q :q_1 = q_1^*, \dots, q_i = q_i^* \}$, then
\begin{equation*}
\max_{\q \in E} \p(O_{1:T}, q_{1:T}) = \frac{\prod_{t=1}^{i-1} \gammat_t(q_t^*, q_{t+1}^*)} {\prod_{t=2}^{i-1} \gammat_t(q_t^*)}.
\end{equation*}
\end{lemma}

\begin{proof}
By Eq.~(\ref{eq:jointp}) we have
\begin{equation*}
\max_{\q \in E} \p(O_{1:T}, q_{1:T}) 
= \max_{\q \in E} \frac{\prod_{t=1}^{T-1} \gammat_t(q_t, q_{t+1})} {\prod_{t=2}^{T-1} \gammat_t(q_t)}  
= \frac{\prod_{t=1}^{i-1} \gammat_t(q_t^*, q_{t+1}^*)} {\prod_{t=2}^{i-1} \gammat_t(q_t^*)} 
  \max_{q_{i+1:T}} \frac{\prod_{t=i}^{T-1} \gammat_t(q_t, q_{t+1})} {\prod_{t=i}^{T-1} \gammat_t(q_t)},
\end{equation*}
then consider the maximisation term
\begin{align*}
\max_{q_{i+1:T}} \frac{\prod_{t=i}^{T-1} \gammat_t(q_t, q_{t+1})} {\prod_{t=i}^{T-1} \gammat_t(q_t)}
&= \max_{q_{i+1:T-1}} \left\{ \frac{\prod_{t=i}^{T-2} \gammat_t(q_t, q_{t+1})} {\prod_{t=i}^{T-1} \gammat_t(q_t)}
   \max_{q_{T}} \gammat_{T-1}(q_{T-1}, q_T) \right\} \\
&= \max_{q_{i+1:T-1}} \left\{ \frac{\prod_{t=i}^{T-2} \gammat_t(q_t, q_{t+1})} {\prod_{t=i}^{T-1} \gammat_t(q_t)}
   \gammat_{T-1}(q_{T-1}) \right\} 
   ~~~ \text{(by Eq.~\ref{eq:maxconsist})} \\
&= \max_{q_{i+1:T-1}} \left\{ \frac{\prod_{t=i}^{T-2} \gammat_t(q_t, q_{t+1})} {\prod_{t=i}^{T-2} \gammat_t(q_t)} \right\}
 = \max_{q_{i+1:T-2}} \left\{ \frac{\prod_{t=i}^{T-3} \gammat_t(q_t, q_{t+1})} {\prod_{t=i}^{T-2} \gammat_t(q_t)}
   \max_{q_{T-1}} \gammat_{T-2}(q_{T-2}, q_{T-1}) \right\} \\
&= \max_{q_{i+1:T-2}} \left\{ \frac{\prod_{t=i}^{T-3} \gammat_t(q_t, q_{t+1})} {\prod_{t=i}^{T-2} \gammat_t(q_t)}
   \gammat_{T-2}(q_{T-2}) \right\}
   ~~~ \text{(by Eq.~\ref{eq:maxconsist})} \\
&= \max_{q_{i+1:T-2}} \left\{ \frac{\prod_{t=i}^{T-3} \gammat_t(q_t, q_{t+1})} {\prod_{t=i}^{T-3} \gammat_t(q_t)} \right\}
 = \max_{q_{i+1:T-3}} \left\{ \frac{\prod_{t=i}^{T-4} \gammat_t(q_t, q_{t+1})} {\prod_{t=i}^{T-3} \gammat_t(q_t)}
   \max_{q_{T-2}} \gammat_{T-3}(q_{T-3}, q_{T-2}) \right\} \\
&= \cdots \\
&= \max_{q_{i+1:i+2}} \left\{ \frac{\prod_{t=i}^{i+1} \gammat_t(q_t, q_{t+1})} {\prod_{t=i}^{i+1} \gammat_t(q_t)} \right\} \\
&= \max_{q_{i+1:i+2}} \left\{ \frac{\gammat_i(q_i^*, q_{i+1}) \cdot \gammat_{i+1}(q_{i+1}, q_{i+2})} 
                                   {\gammat_i(q_i^*) \cdot \gammat_{i+1}(q_{i+1})} \right\}
 = \max_{q_{i+1}} \left\{ \frac{\gammat_i(q_i^*, q_{i+1})} 
                               {\gammat_i(q_i^*) \cdot \gammat_{i+1}(q_{i+1})} 
                          \max_{q_{i+2}} \gammat_{i+1}(q_{i+1}, q_{i+2}) \right\} \\
&= \max_{q_{i+1}} \left\{ \frac{\gammat_i(q_i^*, q_{i+1})} 
                               {\gammat_i(q_i^*) \cdot \gammat_{i+1}(q_{i+1})} \gammat_{i+1}(q_{i+1}) \right\}
   ~~~ \text{(by Eq.~\ref{eq:maxconsist})} \\
&= \max_{q_{i+1}} \left\{ \frac{\gammat_i(q_i^*, q_{i+1})} {\gammat_i(q_i^*)} \right\} \\
&= 1 ~~~ \text{(by Eq.~\ref{eq:maxconsist})}
\end{align*}
and the result follows.
\end{proof}
