\section{Kendall's $\tau$}
\label{sec:kendalltau}

Given two ranks $X$ and $Y$, each with $n$ observations, we define
\begin{itemize}
\item Number of concordant pairs 
      \begin{equation*}
      %C = \sum_{i < j} \left( \mathbbm{1}(X_i < X_j)  \mathbbm{1}(Y_i < Y_j) + \mathbbm{1}(X_i > X_j)  \mathbbm{1}(Y_i > Y_j) \right),
      C = \frac{1}{2} \sum_{i,j} \left( \llb X_i < X_j \rrb  \llb Y_i < Y_j \rrb + \llb X_i > X_j \rrb  \llb Y_i > Y_j \rrb \right),
      \end{equation*}
      where $\llb \cdot \rrb$ is the indicator function and 
      $\sum_{i,j}$ means all unordered pairs $(i, j),~ i,j=1,\dots,n$ are counted twice.

\item Number of discordant pairs 
      \begin{equation*}
      D = \frac{1}{2} \sum_{i,j} \left( \llb X_i < X_j \rrb  \llb Y_i > Y_j \rrb + \llb X_i > X_j \rrb  \llb Y_i < Y_j \rrb \right).
      \end{equation*}

\item Number of ties in $X$
      \begin{equation*}
      T_X = \frac{1}{2} \sum_{i \ne j} \llb X_i = X_j \rrb = \sum_k \frac{t_k (t_k - 1)}{2},
      \end{equation*}
      where $t_k$ is the number of tied values in the $k$-th group of ties for $X$, for example, if
      $X = [12, 2, 1, 12, 2, 2, 1]$, there are $3$ groups of tied values, the first group is the two $12$'s, i.e., $t_1 = 2$;
      the second group is the three $2$'s, i.e., $t_2 = 3$; the third group is the two $1$'s, i.e., $t_3 = 2$. \\
      Similarly, the number of ties in $Y$ is 
      \begin{equation*}
      T_Y = \frac{1}{2} \sum_{i \ne j} \llb Y_i = Y_j \rrb = \sum_k \frac{u_k (u_k - 1)}{2},
      \end{equation*}
      where $u_k$ is the number of tied values in the $k$-th group of ties for $Y$.

\item Number of ties in both $X$ and $Y$
      \begin{equation*}
      T_{XY} = \frac{1}{2} \sum_{i \ne j} \llb X_i = X_j \rrb  \llb Y_i = Y_j \rrb.
      \end{equation*}

\item Number of ties only in $X$
      \begin{equation*}
      T = \frac{1}{2} \sum_{i \ne j} \llb X_i = X_j \rrb  \llb Y_i \ne Y_j \rrb,
      \end{equation*}
      and the number of ties only in $Y$
      \begin{equation*}
      U = \frac{1}{2} \sum_{i \ne j} \llb X_i \ne X_j \rrb  \llb Y_i = Y_j \rrb.
      \end{equation*}
\end{itemize}

Kendall's $\tau$ (version $b$) is defined as~\cite{kendall1945,agresti2010analysis} (and implemented in SciPy~\cite{scipy})
\begin{equation*}
\tau_b = \frac{C - D}{\sqrt{[n(n-1)/2 - T_X] [n(n-1)/2 - T_Y]}} = \frac{C - D}{\sqrt{(C + D + T) (C + D + U)}},
\end{equation*}
where we use equalities 
\begin{align*}
\frac{n(n-1)}{2} &= C + D + T_X + T_Y - T_{XY} \\
T &= T_X - T_{XY} \\
U &= T_Y - T_{XY}
\end{align*}



\subsection{Compare Kendall's $\tau$ with F$_1$ score on points and pairs}
\label{sec:metriccomparison}

Given a prediction $\hat{\mathbf{y}} = (\hat{y}_1, \hat{y}_2, \dots, \hat{y}_K)$ and ground truth $\mathbf{y} = (y_1, y_2, \dots, y_K)$,
for a specific ordering of POIs $(p_1, p_2, \dots, p_{|\mathcal{P}|})$,
we produce two ranks according to $\mathbf{y}$ and $\hat{\mathbf{y}}$,
\begin{align*}
r_i       &= \sum_{j=1}^K (| \mathcal{P} | - j + 1)  \llb p_i = y_j \rrb,~
i = 1, \dots, | \mathcal{P} | \\
\hat{r}_i &= \sum_{j=1}^K (| \mathcal{P} | - j + 1)  \llb p_i = \hat{y}_j \rrb,~ 
i = 1, \dots, | \mathcal{P} |
\end{align*}
where POIs not in $\mathbf{y}$ will have a rank of $0$ in $r$ and similarly in $r$.
Then we have
\begin{align*}
C &= \frac{1}{2} \sum_{i,j} \left(\llb r_i < r_j \rrb  \llb \hat{r}_i < \hat{r}_j \rrb +
     \llb r_i > r_j \rrb  \llb \hat{r}_i > \hat{r}_j \rrb \right), ~i,j = 1, \dots, | \mathcal{P} | \\
D &= \frac{1}{2} \sum_{i,j} \left(\llb r_i < r_j \rrb  \llb \hat{r}_i > \hat{r}_j \rrb +
     \llb r_i > r_j \rrb  \llb \hat{r}_i < \hat{r}_j \rrb \right), \\
T_{\mathbf{y}} &= \frac{1}{2} \sum_{i \ne j} \llb r_i = r_j \rrb 
                = \frac{1}{2} \sum_{i \ne j} \llb r_i = 0 \rrb  \llb r_j = 0 \rrb 
                = \frac{1}{2} \left( |\mathcal{P}| - K \right) \left( |\mathcal{P}| - K - 1 \right), \\ 
T_{\hat{\mathbf{y}}} &= \frac{1}{2} \sum_{i \ne j} \llb \hat{r}_i = \hat{r}_j \rrb
                      = \frac{1}{2} \sum_{i \ne j} \llb \hat{r}_i = 0 \rrb  \llb \hat{r}_j = 0 \rrb
                      = \frac{1}{2} \left( |\mathcal{P}| - K \right) \left( |\mathcal{P}| - K - 1 \right), \\ 
T_{\mathbf{y},\hat{\mathbf{y}}} &= \frac{1}{2} \sum_{i \ne j} \llb r_i = r_j \rrb  \llb \hat{r}_i = \hat{r}_j \rrb
                                 = \frac{1}{2} \sum_{i \ne j} \llb r_i = 0 \rrb  \llb r_j = 0 \rrb 
                                   \llb \hat{r}_i = 0 \rrb  \llb \hat{r}_j = 0 \rrb
                                 = \frac{1}{2} {d(d-1)},
\end{align*}
where $d = \sum_j \llb r_j = 0 \rrb  \llb \hat{r}_j = 0 \rrb$.
Kendall's $\tau$ is
\begin{equation*}
\tau_b = \frac{C - D}{\sqrt{(C + D + T) (C + D + U)}},
\end{equation*}
where $T = T_{\mathbf{y}} - T_{\mathbf{y},\hat{\mathbf{y}}}$ and $U = T_{\hat{\mathbf{y}}} - T_{\mathbf{y},\hat{\mathbf{y}}}$.
As $T_{\y} = T_{\hat\y}$, the denominator of $\tau_b$ is 
\begin{align*}
&\sqrt{(C + D + T)(C + D + U)} \\
&= \sqrt{(C + D + T_{\y} - T_{\y,\hat\y})(C + D + T_{\hat\y} - T_{\y,\hat\y})} \\
&= C + D + T_{\y} - T_{\y,\hat\y} \\
&= \frac{1}{2} \sum_{i,j} \left( \llb r_i < r_j \rrb \llb \hat{r}_i < \hat{r}_j \rrb + \llb r_i > r_j \rrb \llb \hat{r}_i > \hat{r}_j \rrb +
                                 \llb r_i < r_j \rrb \llb \hat{r}_i > \hat{r}_j \rrb + \llb r_i > r_j \rrb \llb \hat{r}_i < \hat{r}_j \rrb \right) +
   T_{\y} - T_{\y,\hat\y} \\
&= \frac{1}{2} \sum_{i,j} \left( \llb r_i < r_j \rrb + \llb r_i > r_j \rrb \right) 
                          \left( \llb \hat{r}_i < \hat{r}_j \rrb + \llb \hat{r}_i > \hat{r}_j \rrb \right) + T_{\y} - T_{\y,\hat\y} \\
&= \frac{1}{2} \sum_{i \ne j} \left( 1 - \llb r_i = r_j \rrb \right) \left( 1 - \llb \hat{r}_i = \hat{r}_j \rrb \right) + T_{\y} - T_{\y,\hat\y} \\
&= \frac{1}{2} \sum_{i \ne j} \left( 1 - \llb r_i = r_j \rrb - \llb \hat{r}_i = \hat{r}_j \rrb + 
                                         \llb r_i = r_j \rrb \llb \hat{r}_i = \hat{r}_j \rrb \right) + 
   \frac{1}{2} \sum_{i \ne j} \llb r_i = r_j \rrb - \frac{1}{2} \sum_{i \ne j} \llb r_i = r_j \rrb \llb \hat{r}_i = \hat{r}_j \rrb \\
&= \frac{1}{2} \sum_{i \ne j} 1 - \frac{1}{2} \sum_{i \ne j} \llb \hat{r}_i = \hat{r}_j \rrb \\
&= \frac{1}{2} |\mathcal{P}|(|\mathcal{P}| - 1) - \frac{1}{2} (|\mathcal{P}| - K) (|\mathcal{P}| - K - 1) \\
&= K|\mathcal{P}| - \frac{K(K + 1)}{2}
\end{align*}
So
\begin{equation*}
\tau_b = \frac{C - D}{K|\mathcal{P}| - K(K + 1)/2}
\end{equation*}

F$_1$ score on points is
\begin{equation*}
F_1 = \frac{1}{K} \sum_i \llb r_i > 0 \rrb  \llb \hat{r}_i > 0 \rrb,
\end{equation*}
and F$_1$ score on pairs is
\begin{equation*}
\text{pairs-F}_1 = \frac{\frac{1}{2} \sum_{i,j} 
                   \llb r_i < r_j \rrb  \llb r_i > 0 \rrb 
                   \llb \hat{r}_i < \hat{r}_j \rrb  \llb \hat{r}_i > 0 \rrb +
                   \frac{1}{2} \sum_{i,j} 
                   \llb r_i > r_j \rrb  \llb r_j > 0 \rrb 
                   \llb \hat{r}_i > \hat{r}_j \rrb  \llb \hat{r}_j > 0 \rrb}{K(K-1)/2}.
\end{equation*}

Define $\bar{r}_i = \llb r_i > 0 \rrb$ and $\bar{\hat{r}}_i = \llb \hat{r}_i > 0 \rrb$,
which means the values of both $\bar{r}_i$ and $\bar{\hat{r}}_i$ are binary, as a result,
the number of concordant pairs between rank $\bar{r}$ and rank $\bar{\hat{r}}$ can be written as
\begin{align*}
\bar{C} &= \frac{1}{2} \sum_{i,j} \left(
           \llb \bar{r}_i < \bar{r}_j \rrb  \llb \bar{\hat{r}}_i < \bar{\hat{r}}_j \rrb +
           \llb \bar{r}_i > \bar{r}_j \rrb  \llb \bar{\hat{r}}_i > \bar{\hat{r}}_j \rrb \right) \\
        &= \frac{1}{2} \sum_{i,j} \left(
           \llb \bar{r}_i = 0 \rrb  \llb \bar{r}_j = 1 \rrb  \llb \bar{\hat{r}}_i = 0 \rrb  \llb \bar{\hat{r}}_j = 1 \rrb +
           \llb \bar{r}_i = 1 \rrb  \llb \bar{r}_j = 0 \rrb  \llb \bar{\hat{r}}_i = 1 \rrb  \llb \bar{\hat{r}}_j = 0 \rrb \right) \\
        &= \frac{1}{2} \sum_{i,j} \left(
           \llb r_i = 0 \rrb  \llb r_j > 0 \rrb  \llb \hat{r}_i = 0 \rrb  \llb \hat{r}_j > 0 \rrb +
           \llb r_i > 0 \rrb  \llb r_j = 0 \rrb  \llb \hat{r}_i > 0 \rrb  \llb \hat{r}_j = 0 \rrb \right) \\
        &= \frac{1}{2} \sum_{i,j} \left(
           \llb r_i < r_j \rrb  \llb r_i = 0 \rrb  \llb \hat{r}_i < \hat{r}_j \rrb  \llb \hat{r}_i = 0 \rrb +
           \llb r_i > r_j \rrb  \llb r_j = 0 \rrb  \llb \hat{r}_i > \hat{r}_j \rrb  \llb \hat{r}_j = 0 \rrb \right) \\
        &= \frac{1}{2} \sum_{i,j} \llb r_i < r_j \rrb  \llb r_i = 0 \rrb  \llb \hat{r}_i < \hat{r}_j \rrb  \llb \hat{r}_i = 0 \rrb +
           \frac{1}{2} \sum_{i,j} \llb r_i > r_j \rrb  \llb r_j = 0 \rrb  \llb \hat{r}_i > \hat{r}_j \rrb  \llb \hat{r}_j = 0 \rrb \\
        &= \frac{1}{2} \sum_{i,j} \llb r_i < r_j \rrb  \llb r_i = 0 \rrb  \llb \hat{r}_i < \hat{r}_j \rrb  \llb \hat{r}_i = 0 \rrb +
           \frac{1}{2} \sum_{i,j} \llb r_j < r_i \rrb  \llb r_j = 0 \rrb  \llb \hat{r}_j < \hat{r}_i \rrb  \llb \hat{r}_j = 0 \rrb \\
        &= \sum_{i,j} \llb r_i < r_j \rrb  \llb r_i = 0 \rrb  \llb \hat{r}_i < \hat{r}_j \rrb  \llb \hat{r}_i = 0 \rrb \\
        &= \sum_{i,j} \llb r_i > r_j \rrb  \llb r_j = 0 \rrb  \llb \hat{r}_i > \hat{r}_j \rrb  \llb \hat{r}_j = 0 \rrb.
\end{align*}

Furthermore, we can rewrite the F$_1$ score on points as 
\begin{align*}
F_1 &= \frac{1}{K} \sum_i \llb r_i > 0 \rrb  \llb \hat{r}_i > 0 \rrb \\
    &= \frac{\frac{1}{K} \sum_{i,j} \llb r_i > r_j \rrb  \llb r_j = 0 \rrb  \llb \hat{r}_i > \hat{r}_j \rrb  \hat{r}_j = 0 \rrb}
            {\sum_j \llb r_j = 0 \rrb  \llb \hat{r}_j = 0 \rrb} ~~ 
            \text{as we repeatedly count the same $i$ for all $r_j = 0$ and $\hat{r}_j = 0$}, \\
    &= \frac{\bar{C}} {dK}.
\end{align*}

We can rewrite the number of concordant pairs as
\begin{align*}
C =& \frac{1}{2} \sum_{i,j} \left(\llb r_i < r_j \rrb  \llb \hat{r}_i < \hat{r}_j \rrb +
     \llb r_i > r_j \rrb  \llb \hat{r}_i > \hat{r}_j \rrb \right), \\
  =& \frac{1}{2} \sum_{i,j} \llb r_i < r_j \rrb  
     \left( \llb r_i > 0 \rrb + \llb r_i = 0 \rrb \right)  
     \llb \hat{r}_i < \hat{r}_j \rrb 
     \left( \llb \hat{r}_i > 0 \rrb + \llb \hat{r}_i = 0 \rrb \right) + \\
   & \frac{1}{2} \sum_{i,j} \llb r_i > r_j \rrb  
     \left( \llb r_j > 0 \rrb + \llb r_j = 0 \rrb \right) 
     \llb \hat{r}_i > \hat{r}_j \rrb 
     \left( \llb \hat{r}_j > 0 \rrb + \llb \hat{r}_j = 0 \rrb \right) \\
  =& \frac{1}{2} \sum_{i,j} \left( \uwave{\llb r_i < r_j \rrb  \llb r_i > 0 \rrb} +
            \llb r_i < r_j \rrb  \llb r_i = 0 \rrb \right)  
     \left( \uwave{\llb \hat{r}_i < \hat{r}_j \rrb  \llb \hat{r}_i > 0 \rrb} + 
            \llb \hat{r}_i < \hat{r}_j \rrb  \llb \hat{r}_i = 0 \rrb \right) + \\
   & \frac{1}{2} \sum_{i,j} \left( \uwave{\llb r_i > r_j \rrb  \llb r_j > 0 \rrb} + 
            \llb r_i > r_j \rrb  \llb r_j = 0 \rrb \right) 
     \left( \uwave{\llb \hat{r}_i > \hat{r}_j \rrb  \llb \hat{r}_j > 0 \rrb} + 
            \llb \hat{r}_i > \hat{r}_j \rrb  \llb \hat{r}_j = 0 \rrb \right) \\
  =& \frac{1}{2} \sum_{i,j} \uwave{\llb r_i < r_j \rrb  \llb r_i > 0 \rrb 
                         \llb \hat{r}_i < \hat{r}_j \rrb  \llb \hat{r}_i > 0 \rrb} +
     \frac{1}{2} \sum_{i,j} \uwave{\llb r_i > r_j \rrb  \llb r_j > 0 \rrb 
                         \llb \hat{r}_i > \hat{r}_j \rrb  \llb \hat{r}_j > 0 \rrb} + \\
   & \frac{1}{2} \sum_{i,j} \left( \uwave{\llb r_i < r_j \rrb  \llb r_i > 0 \rrb} 
                         \llb \hat{r}_i < \hat{r}_j \rrb  \llb \hat{r}_i = 0 \rrb + 
                         \llb r_i < r_j \rrb  \llb r_i = 0 \rrb  
                         \llb \hat{r}_i < \hat{r}_j \rrb \right) + \\ 
   & \frac{1}{2} \sum_{i,j} \left( \uwave{\llb r_i > r_j \rrb  \llb r_j > 0 \rrb} 
                         \llb \hat{r}_i > \hat{r}_j \rrb  \llb \hat{r}_j = 0 \rrb +
                         \llb r_i > r_j \rrb  \llb r_j = 0 \rrb 
                         \llb \hat{r}_i > \hat{r}_j \rrb \right) \\
  =& ~\text{pairs-F}_1  \frac{K(K-1)}{2}~ + \\
   & \frac{1}{2} \sum_{i,j} \left( \uwave{\llb r_i < r_j \rrb  \llb r_i > 0 \rrb} 
                         \llb \hat{r}_i < \hat{r}_j \rrb  \llb \hat{r}_i = 0 \rrb + 
                         \llb r_i < r_j \rrb  \llb r_i = 0 \rrb  
                         \llb \hat{r}_i < \hat{r}_j \rrb \right) + \\ 
   & \frac{1}{2} \sum_{i,j} \left( \uwave{\llb r_i > r_j \rrb  \llb r_j > 0 \rrb} 
                         \llb \hat{r}_i > \hat{r}_j \rrb  \llb \hat{r}_j = 0 \rrb +
                         \llb r_i > r_j \rrb  \llb r_j = 0 \rrb 
                         \llb \hat{r}_i > \hat{r}_j \rrb \right).
\end{align*}
We can simplify $C-D$ and $C+D$ in a similar manner,
\begin{align*}
C-D &= \frac{1}{2} \sum_{i,j} \left( \llb r_j > 0 \rrb (1 - \llb r_i > r_j \rrb) - \llb r_i > 0 \rrb (1 - \llb r_i < r_j \rrb) \right)
       \left( \llb \hat{r}_j > 0 \rrb (1 - \llb \hat{r}_i > \hat{r}_j \rrb) - \llb \hat{r}_i > 0 \rrb (1 - \llb \hat{r}_i < \hat{r}_j \rrb) \right) \\
C+D &= \frac{1}{2} \sum_{i,j} \left( \llb r_j > 0 \rrb (1 + \llb r_i > r_j \rrb) + \llb r_i > 0 \rrb (1 + \llb r_i < r_j \rrb) \right)
       \left( \llb \hat{r}_j > 0 \rrb (1 + \llb \hat{r}_i > \hat{r}_j \rrb) + \llb \hat{r}_i > 0 \rrb (1 + \llb \hat{r}_i < \hat{r}_j \rrb) \right)
\end{align*}
