\section{Proof of Lemma~\ref{lm:rank2clf}}

First, we can approximate the empirical risk $R_\textsc{rank}$ (with the exponential surrogate) as follows:
\begin{equation*}
\begin{aligned}
R_\textsc{rank}^\textsc{exp}(\uptheta)
&= \frac{1}{N} \sum_{u=1}^U \sum_{i \in P_u} \frac{1}{M_-^i} \sum_{m': y_{m'}^i = 0} \exp \left( -\min_{m: y_m^i = 1} f(m, u, i) + f(m', u, i) \right) \\
&= \frac{1}{N} \sum_{u=1}^U \sum_{i \in P_u} \frac{1}{M_-^i} \exp \left( -\min_{m: y_m^i = 1} f(m, u, i) \right) 
   \sum_{m': y_{m'}^i = 0} \exp \left( f(m', u, i) \right) \\
&\approx \frac{1}{N} \sum_{u=1}^U \sum_{i \in P_u} \frac{1}{M_-^i} \exp \left( \frac{1}{p} \log \sum_{m: y_m^i = 1} e^{-p f(m, u, i)} \right)
   \sum_{m': y_{m'}^i = 0} \exp \left( f(m', u, i) \right) \\
&= \frac{1}{N} \sum_{u=1}^U \sum_{i \in P_u} \frac{1}{M_-^i} \left( \sum_{m: y_m^i = 1} e^{-p f(m, u, i)} \right)^\frac{1}{p} 
   \sum_{m': y_{m'}^i = 0} e^{f(m', u, i)} \\
&= \frac{1}{N} \sum_{u=1}^U \sum_{i \in P_u} \frac{1}{M_-^i} \left( \left( \sum_{m': y_{m'}^i = 0} e^{f(m', u, i)} \right)^p 
   \sum_{m: y_m^i = 1} e^{-p f(m, u, i)} \right)^\frac{1}{p} \\
&= \frac{1}{N} \sum_{u=1}^U \sum_{i \in P_u} \frac{1}{M_-^i} \left( 
   \sum_{m: y_m^i = 1} e^{-p f(m, u, i)} \left( \sum_{m': y_{m'}^i = 0} e^{f(m', u, i)} \right)^p \right)^\frac{1}{p} \\
&= \frac{1}{N} \sum_{u=1}^U \sum_{i \in P_u} \frac{1}{M_-^i} \left( 
   \sum_{m: y_m^i = 1} \left( \sum_{m': y_{m'}^i = 0} e^{- \left( f(m, u, i) - f(m', u, i) \right)} \right)^p \right)^\frac{1}{p} \\
&= \widetilde R_\textsc{rank}.
\end{aligned}
\end{equation*}

Let $R_\textsc{clf}$ be the following classification risk:
\begin{equation*}
R_\textsc{clf} 
= \frac{1}{N} \sum_{u=1}^U \sum_{i \in P_u} \left( 
  \frac{1}{p M_+^i} \sum_{m: y_m^i = 1} e^{-p f(m, u, i)} 
  + \frac{1}{M_-^i} \sum_{m': y_{m'}^i = 0} e^{f(m', u, i)} \right),
\end{equation*}

Let $\uptheta^* \in \argmin_{\uptheta} R_\textsc{clf}$ (assuming minimisers exist),
We want to prove that $\uptheta^* \in \argmin_{\uptheta} \widetilde R_\textsc{rank}$.

\begin{proof}
We following the proof technique in~\cite{ertekin2011equivalence}
by first introducing a constant feature $1$ for each song,
without loss of generality, let the first feature of $\x_m, \, m \in \{1,\dots,M\}$ be the constant feature, \ie $x_m^0 = 1$.
We can show that
$\frac{\partial \, R_\textsc{clf}} {\partial \, \uptheta} = 0$ implies
$\frac{\partial \, \widetilde R_\textsc{rank}} {\partial \, \uptheta} = 0$,
which means minimisers of $R_\textsc{clf}$ also minimise $\widetilde R_\textsc{rank}$.

Let 
\begin{equation*}
\begin{aligned}
0 
&= \frac{\partial \, R_\textsc{clf}} {\partial \, \alpha_i^0}
&= \frac{1}{N} \left( 
   \frac{1}{p M_+^i} \sum_{m: y_m^i = 1} e^{-p f(m, u, i)} (-p)
   + \frac{1}{M_-^i} \sum_{m': y_{m'}^i = 0} e^{f(m', u, i)} \right),
\ \forall i \in P_u, \, u \in \{1,\dots,U\},
\end{aligned}
\end{equation*}
we have
\begin{equation}
\label{eq:eq1}
\frac{1}{M_+^i} \sum_{m: y_m^i = 1} e^{-p f(m, u, i)} \Bigg|_{\uptheta = \uptheta^*}
= \frac{1}{M_-^i} \sum_{m': y_{m'}^i = 0} e^{f(m', u, i)} \Bigg|_{\uptheta = \uptheta^*}, 
\ \forall i \in P_u, \, u \in \{1,\dots,U\},
\end{equation}

Further, let
\begin{equation*}
\zero 
= \frac{\partial \, R_\textsc{clf}} {\partial \, \alphabm_i} 
= \frac{1}{N} \left( 
   \frac{1}{p M_+^i} \sum_{m: y_m^i = 1} e^{-p f(m, u, i)} (-p \x_m)
   + \frac{1}{M_-^i} \sum_{m': y_{m'}^i = 0} e^{f(m', u, i)} \x_{m'} \right),
\ \forall i \in P_u, \, u \in \{1,\dots,U\},
\end{equation*}
we have
\begin{equation}
\label{eq:eq2}
\frac{1}{M_+^i} \sum_{m: y_m^i = 1} e^{-p f(m, u, i)} \x_m \Bigg|_{\uptheta = \uptheta^*}
= \frac{1}{M_-^i} \sum_{m': y_{m'}^i = 0} e^{f(m', u, i)} \x_{m'} \Bigg|_{\uptheta = \uptheta^*},
\ \forall i \in P_u, \, u \in \{1,\dots,U\}.
\end{equation}

Note that $\forall i \in P_u, \, u \in \{1,\dots,U\}$,
\begin{equation}
\label{eq:eq3}
\resizebox{\textwidth}{!}{$
\begin{aligned}
&\frac{\partial \, \widetilde R_\textsc{rank}} {\partial \, \alphabm_i} \Bigg|_{\uptheta = \uptheta^*} \\
&= \frac{1}{N M_-^i} \left[
   \frac{1}{p} \left( \sum_{m: y_m^i = 1} e^{-p f(m, u, i)} \right)^{\frac{1}{p} - 1} 
   \sum_{m: y_m^i = 1} e^{-p f(m, u, i)} (-p \x_m) 
   \sum_{m': y_{m'}^i = 0} e^{f(m', u, i)} + 
   \left( \sum_{m: y_m^i = 1} e^{-p f(m, u, i)} \right)^\frac{1}{p}
   \sum_{m': y_{m'}^i = 0} e^{f(m', u, i)} \x_{m'} \right] \\
&= \frac{-1}{N M_-^i}
   \left( \sum_{m: y_m^i = 1} e^{-p f(m, u, i)} \right)^{\frac{1}{p} - 1} 
   \left[
   \sum_{m: y_m^i = 1} e^{-p f(m, u, i)} \x_m 
   \sum_{m': y_{m'}^i = 0} e^{f(m', u, i)} -
   \sum_{m: y_m^i = 1} e^{-p f(m, u, i)}
   \sum_{m': y_{m'}^i = 0} e^{f(m', u, i)} \x_{m'} \right] \\
&= \frac{-1}{N M_-^i}
   \left( \sum_{m: y_m^i = 1} e^{-p f(m, u, i)} \right)^{\frac{1}{p} - 1} 
   \left[
   \sum_{m: y_m^i = 1} e^{-p f(m, u, i)} \x_m 
   \frac{M_-^i}{M_+^i} \sum_{m: y_m^i = 1} e^{-p f(m, u, i)} -
   \sum_{m: y_m^i = 1} e^{-p f(m, u, i)}
   \sum_{m': y_{m'}^i = 0} e^{f(m', u, i)} \x_{m'} \right] \ (\text{by Eq.~\ref{eq:eq1}}) \\
&= \frac{-1}{N M_-^i}
   \left( \sum_{m: y_m^i = 1} e^{-p f(m, u, i)} \right)^\frac{1}{p}
   \left[
   \sum_{m: y_m^i = 1} \frac{M_-^i}{M_+^i} e^{-p f(m, u, i)} \x_m -
   \sum_{m': y_{m'}^i = 0} e^{f(m', u, i)} \x_{m'} \right] \\
&= \zero \ (\text{by Eq.~\ref{eq:eq2}}).
\end{aligned}
$}
\end{equation}

Let 
\begin{equation*}
h(u, i) 
= \frac{1}{N M_-^i} \left( \sum_{m: y_m^i = 1} e^{-p f(m, u, i)} \right)^\frac{1}{p} 
  \sum_{m': y_{m'}^i = 0} e^{f(m', u, i)},
\ \forall i \in P_u, \, u \in \{1,\dots,U\}.
\end{equation*}
then by Eq.~(\ref{eq:eq3}), we have
\begin{equation}
\label{eq:eq4}
\frac{\partial \, h(u, i)}{\partial \, \alphabm_i} \Bigg|_{\uptheta = \uptheta^*} = \zero,
\ \forall i \in P_u, \, u \in \{1,\dots,U\}.
\end{equation}

Note that $\forall u \in \{1,\dots,U\}$,
by Eq.~(\ref{eq:eq4})
\begin{equation}
\label{eq:eq5}
\frac{\partial \, \widetilde R_\textsc{rank}} {\partial \, \betabm_u} \Bigg|_{\uptheta = \uptheta^*} 
= \sum_{i \in P_u} \frac{\partial \, h(u, i)}{\partial \, \betabm_u}  \Bigg|_{\uptheta = \uptheta^*}
= \sum_{i \in P_u} \frac{\partial \, h(u, i)}{\partial \, \alphabm_i} \Bigg|_{\uptheta = \uptheta^*}
= \zero,
\end{equation}
and
\begin{equation}
\label{eq:eq6}
\frac{\partial \, \widetilde R_\textsc{rank}} {\partial \, \bmu} \Bigg|_{\uptheta = \uptheta^*} 
= \sum_{u=1}^U \sum_{i \in P_u} \frac{\partial \, h(u, i)}{\partial \, \bmu} \Bigg|_{\uptheta = \uptheta^*}
= \sum_{u=1}^U \sum_{i \in P_u} \frac{\partial \, h(u, i)}{\partial \, \alphabm_i} \Bigg|_{\uptheta = \uptheta^*}
= \zero.
\end{equation}

Finally, by Eq.~(\ref{eq:eq3}), (\ref{eq:eq5}), (\ref{eq:eq6}), $\uptheta^* \in \argmin_{\uptheta} \widetilde R_\textsc{rank}$.

\end{proof}
