\begin{equation}
\label{eq:primal}
\begin{aligned}
&\min_{\V, \W, \mubm} \ \frac{\lambda}{2} \left( \frac{1}{U} \sum_{u=1}^U \bv_u^\top \bv_u 
     + \frac{1}{N} \sum_{i=1}^N \w_i^\top \w_i + \mubm^\top \mubm \right) \\
& \hspace{4em}
     + \frac{1}{N} \sum_{i=1}^N \frac{1}{M_i^+} \sum_{m: y_i^m = 1} \ell \left( (\bv_{u(i)} + \w_i + \mubm)^\top \x^m 
     - \max_{n: y_i^n = 0} (\bv_{u(i)} + \w_i + \mubm)^\top \x^n \right).
\end{aligned}
\end{equation}

Let 
\begin{equation*}
\begin{aligned}
f_0(\V, \W, \mubm, \xibm) &= \frac{\lambda}{2} \left( \frac{1}{U} \sum_{u=1}^U \bv_u^\top \bv_u 
     + \frac{1}{N} \sum_{i=1}^N \w_i^\top \w_i + \mubm^\top \mubm \right) \\
& \quad \ 
     + \frac{1}{N} \sum_{i=1}^N \frac{1}{M_i^+} \sum_{m: y_i^m = 1} 
       \ell \left( (\bv_{u(i)} + \w_i + \mubm)^\top \x^m - \xi_i \right) \\
f_{i,n} (\V, \W, \mubm, \xibm) &= (\bv_{u(i)} + \w_i + \mubm)^\top \x^n - \xi_i, \
i \in \{1,\dots,N\}, \, n \in \{1,\dots,M\} \ \mathrm{and} \ y_i^n = 0.
\end{aligned}
\end{equation*}

Problem (\ref{eq:primal}) is equivalent to 
\begin{equation}
\label{eq:stdopt}
\begin{aligned}
\min_{\V, \W, \mubm, \xibm} \ & f_0(\V, \W, \mubm, \xibm) \\
s.t. \quad & f_{i,n}(\V, \W, \mubm, \xibm) \le 0, \
i \in \{1,\dots,N\}, \, n \in \{1,\dots,M\} \ \mathrm{and} \ y_i^n = 0.
\end{aligned}
\end{equation}

For $\beta_i^n \ge 0$, the \emph{Lagrangian} of (\ref{eq:stdopt}) is
\begin{equation*}
\begin{aligned}
L(\V, \W, \mubm, \xibm, \betabm) 
&= f_0(\V, \W, \mubm, \xibm) + \sum_{i=1}^N \sum_{n: y_i^n = 0} \beta_i^n f_{i,n} (\V, \W, \mubm, \xibm).
\end{aligned}
\end{equation*}

Note that the conjugate of the conjugate of a convex function is itself, \ie $f(\z) = f^{**}(\z) = \sup_\y \left(\z^\top \y - f^*(\y) \right)$, we have
\begin{equation*}
\begin{aligned}
\ell \left( (\bv_{u(i)} + \w_i + \mubm)^\top \x^m - \xi_i \right)
&= \sup_{\alpha_i^m} \left[ \left( (\bv_{u(i)} + \w_i + \mubm)^\top \x^m - \xi_i \right) \alpha_i^m - \ell^*(\alpha_i^m) \right],
\end{aligned}
\end{equation*}
where $\ell^*$ is the convex conjugate of surrogate loss $\ell$.

Let
\begin{equation*}
\begin{aligned}
g(\V, \W, \mubm, \xibm, \alphabm, \betabm)
&= \frac{\lambda}{2} \left( \frac{1}{U} \sum_{u=1}^U \bv_u^\top \bv_u 
     + \frac{1}{N} \sum_{i=1}^N \w_i^\top \w_i + \mubm^\top \mubm \right) \\
& \hspace{2em}
     + \sum_{i=1}^N \frac{1}{N M_i^+} \sum_{m: y_i^m = 1} \left( (\bv_{u(i)} + \w_i + \mubm)^\top \x^m - \xi_i \right) \alpha_i^m \\
& \hspace{2em}
     + \sum_{i=1}^N \sum_{n: y_i^n = 0} \beta_i^n \left( (\bv_{u(i)} + \w_i + \mubm)^\top \x^n - \xi_i \right), \\
r(\alphabm)
&= \sum_{i=1}^N \frac{1}{N M_i^+} \sum_{m: y_i^m = 1} \ell^*(\alpha_i^m),
\end{aligned}
\end{equation*}
then 
\begin{equation*}
\begin{aligned}
L(\V, \W, \mubm, \xibm, \alphabm, \betabm) 
= \sup_\alphabm \left[ g(\V, \W, \mubm, \xibm, \alphabm, \betabm) - r(\alphabm) \right].
\end{aligned}
\end{equation*}

Assuming strong duality, the \emph{Lagrangian dual function} of (\ref{eq:stdopt}) is
\begin{equation*}
\begin{aligned}
\inf_{\V, \W, \mubm, \xibm} L(\V, \W, \mubm, \xibm, \alphabm, \betabm) 
&= \inf_{\V, \W, \mubm, \xibm} \sup_\alphabm \left[ g(\V, \W, \mubm, \xibm, \alphabm, \betabm) - r(\alphabm) \right] \\
&= \sup_\alphabm \inf_{\V, \W, \mubm, \xibm} \left[ g(\V, \W, \mubm, \xibm, \alphabm, \betabm) - r(\alphabm) \right] \\
&= \sup_\alphabm \left[ \inf_{\V, \W, \mubm, \xibm} g(\V, \W, \mubm, \xibm, \alphabm, \betabm) - r(\alphabm) \right] \\
&= \max_\alphabm \left[ \min_{\V, \W, \mubm, \xibm} g(\V, \W, \mubm, \xibm, \alphabm, \betabm) - r(\alphabm) \right].
\end{aligned}
\end{equation*}

To solve the inner (unconstrained) minimisation, let
\begin{equation*}
\begin{aligned}
\zero &= \frac{\partial g}{\partial \bv_u} 
       = \frac{\lambda}{U} \bv_u 
         + \sum_{i \in P_u} \left( \frac{1}{N M_i^+} \sum_{m: y_i^m = 1} \alpha_i^m \x^m + \sum_{n: y_i^n = 0} \beta_i^n \x^n \right) \\
\zero &= \frac{\partial g}{\partial \w_i}
       = \frac{\lambda}{N} \w_i + \frac{1}{N M_i^+} \sum_{m: y_i^m = 1} \alpha_i^m \x^m + \sum_{n: y_i^n = 0} \beta_i^n \x^n \\
\zero &= \frac{\partial g}{\partial \mubm} 
       = \lambda \mubm + \sum_{i=1}^N \left( \frac{1}{N M_i^+} \sum_{m: y_i^m = 1} \alpha_i^m \x^m + \sum_{n: y_i^n = 0} \beta_i^n \x^n \right) \\
0     &= \frac{\partial g}{\partial \xi_i}
       = - \frac{1}{N M_i^+} \sum_{m: y_i^m = 1} \alpha_i^m - \sum_{n: y_i^n = 0} \beta_i^n \\
\end{aligned}
\end{equation*}
where $P_u$ denotes the indices of playlists from user $u$.

To simplify the notation, let $\Thetabm \in \R^{M \times N}$ such that
\begin{equation*}
\theta_i^m = 
\begin{cases}
    \frac{\alpha_i^m}{N M_i^+}, & y_i^m = 1 \\
    \beta_i^m, & y_i^m = 0, \ i \in \{1,\dots,N\}, \, m \in \{1,\dots,M\},
\end{cases}
\end{equation*}
then we have
\begin{equation*}
\begin{aligned}
\bv_u^\top &= -\frac{U}{\lambda} \sum_{i \in P_u} \thetabm_i^\top \X \\
\w_i^\top  &= -\frac{N}{\lambda} \thetabm_i^\top \X \\
\mubm^\top &= -\frac{1}{\lambda} \sum_{i=1}^N \thetabm_i^\top \X \\
\thetabm_i^\top \one_M &= 0
\end{aligned}
\end{equation*}

Thus, we have
\begin{equation*}
\begin{aligned}
&\min_{\V, \W, \mubm, \xibm} g(\V, \W, \mubm, \xibm, \alphabm, \betabm) \\
&= \frac{\lambda}{2} \left( \frac{1}{U} \sum_{u=1}^U \bv_u^\top \bv_u 
     + \frac{1}{N} \sum_{i=1}^N \w_i^\top \w_i + \mubm^\top \mubm \right) \\
& \hspace{2em}
     + \sum_{i=1}^N \left( 
       \sum_{m: y_i^m = 1} \frac{\alpha_i^m}{N M_i^+} (\bv_{u(i)} + \w_i + \mubm)^\top \x^m 
     + \sum_{n: y_i^n = 0} \beta_i^n (\bv_{u(i)} + \w_i + \mubm)^\top \x^n \right) \\
& \hspace{2em}
     - \sum_{i=1}^N \xi_i \left( \sum_{m: y_i^m = 1} \frac{\alpha_i^m}{N M_i^+} + \sum_{n: y_i^n = 0} \beta_i^n \right) \\
%   + \sum_{u=1}^U \sum_{i \in P_u} \sum_{m = 1}^M \theta_i^m \left( (\bv_u + \w_i + \mubm)^\top \x^m - \xi_i \right) \\
&= \frac{\lambda}{2} \left( \frac{1}{U} \sum_{u=1}^U \bv_u^\top \bv_u 
     + \frac{1}{N} \sum_{i=1}^N \w_i^\top \w_i + \mubm^\top \mubm \right)
     + \sum_{i=1}^N \sum_{m=1}^M \theta_i^m (\bv_{u(i)} + \w_i + \mubm)^\top \x^m \\
&= \frac{\lambda}{2} \left( \frac{1}{U} \sum_{u=1}^U \bv_u^\top \bv_u 
     + \frac{1}{N} \sum_{i=1}^N \w_i^\top \w_i + \mubm^\top \mubm \right)
     + \sum_{i=1}^N (\bv_{u(i)} + \w_i + \mubm)^\top \left( \sum_{m=1}^M \theta_i^m \x^m \right) \\
&= \frac{\lambda}{2} \left( \frac{1}{U} \sum_{u=1}^U \bv_u^\top \bv_u 
     + \frac{1}{N} \sum_{i=1}^N \w_i^\top \w_i + \mubm^\top \mubm \right)
     + \sum_{i=1}^N (\bv_{u(i)} + \w_i + \mubm)^\top \left( \thetabm_i^\top \X \right) \\
&= \frac{\lambda}{2} \left( \frac{1}{U} \sum_{u=1}^U \bv_u^\top \bv_u 
     + \frac{1}{N} \sum_{i=1}^N \w_i^\top \w_i + \mubm^\top \mubm \right)
     + \sum_{i=1}^N \bv_{u(i)}^\top \left( \thetabm_i^\top \X \right) 
     + \sum_{i=1}^N \w_i^\top \left( \thetabm_i^\top \X \right) 
     + \mubm^\top \left( \sum_{i=1}^N \thetabm_i^\top \X \right) \\
&= \frac{\lambda}{2} \left( \frac{1}{U} \sum_{u=1}^U \bv_u^\top \bv_u 
     + \frac{1}{N} \sum_{i=1}^N \w_i^\top \w_i + \mubm^\top \mubm \right)
     + \sum_{u=1}^U \sum_{i \in P_u} \bv_u^\top \left( \thetabm_i^\top \X \right) 
     - \frac{\lambda}{N} \sum_{i=1}^N \w_i^\top \w_i 
     + \mubm^\top \left( \sum_{i=1}^N \thetabm_i^\top \X \right) \\
\end{aligned}
\end{equation*}
